{
 "cells": [
  {
   "cell_type": "markdown",
   "metadata": {},
   "source": [
    "### 1) Episode-based REPS\n",
    "\n",
    "**Optimization Problem**\n",
    "\\begin{align}\n",
    "\\max_{\\pi}  &&&\\int \\pi(\\theta) \\mathcal{R}(\\theta) d\\theta \\\\\n",
    "\\text{s.t.} &&& D_{KL}(\\pi_{\\theta}, q(\\theta)) = \\int \\pi(\\theta) \\log \\frac{\\pi(\\theta)}{q(\\theta)} d \\theta - \\epsilon \\leq 0  \\\\\n",
    "&&& \\int \\pi(\\theta) d\\theta - 1 = 0\n",
    "\\end{align}\n",
    "\n",
    "**Lagrange Function**\n",
    "$$\n",
    "L(\\pi_{\\theta}, \\eta, v) = \\int \\pi(\\theta) \\mathcal{R}(\\theta) d\\theta  + \\eta \\left( \\epsilon -  \\int \\pi(\\theta) \\log \\frac{\\pi(\\theta)}{q(\\theta)} d \\theta\\right) + v \\left(1 - \\int \\pi(\\theta) d\\theta \\right)\n",
    "$$\n",
    "\n"
   ]
  },
  {
   "cell_type": "markdown",
   "metadata": {},
   "source": [
    "### 2) Step-based REPS\n",
    "\n",
    "**2.1 Optimization Problem**\n",
    "\\begin{align}\n",
    "\\max_{\\pi, \\mu^{\\pi}}  &&& J(\\pi) = \\sum_{s, a}\\mu^{\\pi}(s) \\pi(a|s) \\mathcal{R} \\\\\n",
    "\\text{s.t.} &&& \\sum_{s, a} \\mu^{\\pi}(s) \\pi(a|s) \\log{\\frac{\\mu^{\\pi}(s)\\pi(a|s)}{q(s,a)}} \\leq \\epsilon \\\\\n",
    "&&& \\sum_{s'} \\mu^{\\pi}(s')\\phi_{s'} = \\sum_{s, a, s'} \\mu^{\\pi}(s) \\pi(a|s)\\mathcal{P}_{ss'}^a\\phi_{s'} \\\\\n",
    "&&& \\sum_{s, a}\\mu^{\\pi}(s)\\pi(a|s)=1\n",
    "\\end{align}\n",
    "\n",
    "**2.2 Lagrangian Function**\n",
    "\n",
    "\\begin{align}\n",
    "L(p_{sa}, \\eta, \\theta, \\lambda) &= \\left(\\sum_{s, a}p_{sa}\\mathcal{R}_s^a \\right) + \\eta \\left( \\epsilon - \\sum_{s, a} p_{sa} \\log{\\frac{p_{sa}}{q_{sa}}} \\right) + \\sum_{s'} \\theta^T \\left(  \\sum_{a'}p_{s'a'}\\phi_{s'} - \\sum_{s,a}p_{sa}\\mathcal{p}_{ss'}^a \\phi_{s'}  \\right) + \\lambda \\left( 1 - \\sum_{s,a}p_{sa} \\right) \\\\\n",
    "& = \\sum_{s,a}p_{sa} \\left(\\mathcal{R}_s^{a} - \\eta \\log{\\frac{p_{sa}}{q_{sa}}} - \\lambda - \\theta_s^T\\phi_s + \\sum_{s'}\\mathcal{p}_{ss'}^a \\theta_{s'}^{T}\\phi_{s'} \\right) + \\eta \\epsilon + \\lambda\n",
    "\\end{align}\n",
    "\n",
    "> * for brevity of the derivations, we denote $ p_{sa} = \\mu^{\\pi}(s)\\pi(a|s) \\quad \\mu^{\\pi}(s) = \\sum_a p_{sa}$\n",
    "* $\\eta$, $\\theta$, $\\lambda$ denote the Lagrangian multipliers\n",
    "* we can substitute $V_s = \\theta^T \\phi_s$\n",
    "* differentiate\n",
    "\\begin{align}\n",
    "\\partial_{p_{sa}}L(p_{sa}, \\eta, \\theta, \\lambda) &= \\mathcal{R}_{s}^{a} - \\eta(\\log{\\frac{p_{sa}}{q_{sa}}} + 1 ) - \\lambda + \\sum_{s'}\\mathcal{P}_{ss'}^{a}V_{s'} - V_s = 0 \\\\\n",
    "p_{sa} & = q_{sa}\\exp{\\left( \\frac{1}{\\eta} (\\mathcal{R}_s^a + \\sum_{s'}\\mathcal{p}_{ss'}^a V_{s'} - V_s) \\right)} \\exp{\\left(-1 -\\frac{\\lambda}{\\eta}\\right)} \\\\\n",
    "\\sum_{s,a}p_{sa} = 1 & \\Rightarrow \\exp{(-1 -\\frac{\\lambda}{\\eta})} = \\left(\\sum_{s,a}q_{sa}\\exp{(\\frac{1}{\\eta} (R_s^a + \\sum_{s'}\\mathcal{p}_{ss'}^a V_{s'} - V_s))} \\right)^{-1} \n",
    "\\end{align}\n",
    "* result \n",
    "$$\n",
    "p_{sa} = \\frac{q_{sa}\\exp{\\left( \\frac{1}{\\eta} (R_s^a + \\sum_{s'}\\mathcal{p}_{ss'}^a V_{s'} - V_s) \\right)}}{\\sum_{s,a}q_{sa}\\exp{\\left(\\frac{1}{\\eta} (R_s^a + \\sum_{s'}\\mathcal{p}_{ss'}^a V_{s'} - V_s)\\right)}} \\quad\\leftarrow \\quad \\text{Closed-form solution}\n",
    "$$\n",
    "\n",
    "**2.3 Lagrangian dual function**\n",
    "\\begin{align}\n",
    "g(\\eta, v) = \\eta \\epsilon + \\eta \\log{\\sum_{s,a}q(s,a) \\exp{\\left( \\frac{\\delta_v(s,a)}{\\eta}\\right)}}\n",
    "\\end{align}\n",
    "\n",
    "> * Step 0:\n",
    "$$\n",
    "\\left\\{\n",
    "\\begin{array}{lr} \n",
    "L(p_{sa}, \\eta, \\theta, \\lambda)   = \\sum_{s,a}p_{sa} \\left(\\mathcal{R}_s^{a} - \\eta \\log{\\frac{p_{sa}}{q_{sa}}} - \\lambda -  V_{s}+ \\sum_{s'}\\mathcal{p}_{ss'}^a V_{s'}\\right) + \\eta \\epsilon + \\lambda \\quad &&(1)\\\\\n",
    "p_{sa}  = q_{sa}\\exp{\\left( \\frac{1}{\\eta} (\\mathcal{R}_s^a + \\sum_{s'}\\mathcal{p}_{ss'}^a V_{s'} - V_s) \\right)} \\exp{\\left(-1 -\\frac{\\lambda}{\\eta}\\right)} \\quad &&(2) \\\\\n",
    "\\exp{(-1 -\\frac{\\lambda}{\\eta})}  = \\left(\\sum_{s,a}q_{sa}\\exp{(\\frac{1}{\\eta} (R_s^a + \\sum_{s'}\\mathcal{p}_{ss'}^a V_{s'} - V_s))} \\right)^{-1}  \\quad &&(3)\\\\\n",
    "\\end{array} \n",
    "\\right.\n",
    "$$\n",
    "* Step 1, insert Equation (2) into the $\\log{p_{sa}}$ term of Equation (1), denote $\\delta(s,a)=\\mathcal{R}_s^{a}+ \\sum_{s'}\\mathcal{p}_{ss'}^a V_{s'} -  V_{s}$\n",
    "\\begin{align}\n",
    "L(\\eta, \\lambda) &= \\sum_{s,a}p_{sa} \\left(\\delta(s,a) - \\eta \\log{\\frac{p_{sa}}{q_{sa}}} - \\lambda\\right) + \\eta \\epsilon + \\lambda \\\\\n",
    "& = \\sum_{s,a}p_{sa} \\left(\\delta(s,a) - \\eta \\log{ \\left( \\frac{q_{sa}}{q_{sa}} \\exp(\\frac{\\delta(s,a)}{\\eta})\\exp(\\frac{-\\eta -\\lambda}{\\eta} \\right)} - \\lambda\\right) + \\eta \\epsilon + \\lambda  \\\\\n",
    "& = \\sum_{s,a}p_{sa} \\left(\\delta(s,a) - \\eta \\left( \\frac{\\delta(s,a)}{\\eta} + \\frac{-\\eta -\\lambda}{\\eta} \\right) - \\lambda\\right) + \\eta \\epsilon + \\lambda \\\\\n",
    "& = \\sum_{s,a}p_{sa} \\left(\\delta(s,a) - \\delta(s,a) + \\eta + \\lambda- \\lambda\\right) + \\eta \\epsilon + \\lambda \\\\\n",
    "& = \\sum_{s,a}p_{sa}\\eta  + \\eta \\epsilon + \\lambda \\\\\n",
    "& = 1 \\cdot \\eta  + \\eta \\epsilon + \\lambda \\\\\n",
    "& = \\eta \\epsilon + \\eta \\log{\\exp{\\frac{\\eta+\\lambda}{\\eta}}} \\quad (4)\n",
    "\\end{align}\n",
    "* Step 2, insert Equation (3) into equation (4), the dual function therefore depends on $\\eta$ and $v$,\n",
    "\\begin{align}\n",
    "g(\\eta, v) = \\eta \\epsilon + \\eta \\log{\\sum_{s,a}q(s,a) \\exp{\\left( \\frac{\\delta_v(s,a)}{\\eta}\\right)}}\n",
    "\\end{align}\n",
    "\n",
    "**Optimizing the Dual-Function**\n",
    "\n",
    "The dual function is in log-sum-exp form, and therefore convex in $v$. We have one inequality constraint in the original optimization problem. \n",
    "\\begin{align}\n",
    "\\underset{\\eta, v}{\\text{min}} \\quad g(\\eta, v) &= \\eta \\epsilon + \\eta \\log{\\sum_{s,a}q(s,a) \\exp{\\left( \\frac{\\delta_v(s,a)}{\\eta}\\right)}} \\\\\n",
    "\\text{s.t.:} \\quad & \\eta \\geq 0\n",
    "\\end{align}"
   ]
  },
  {
   "cell_type": "markdown",
   "metadata": {},
   "source": [
    "### 3)f-divergence constrained policy optimization\n",
    "\n",
    "**3.1 Optimization Problem**\n",
    "\n",
    "\\begin{equation*}\n",
    "\\begin{aligned}[c]\n",
    "\\max_{\\theta} \\quad & J(\\pi_\\theta) = \\mathbb{\\hat{E}}\\left[ \\frac{\\pi_{\\theta}(a_t | s_t)}{\\pi_{\\theta_{old}}(a_t | s_t)} \\hat{A}_t\\right] \\\\\n",
    "\\text{s.t.: } \\quad & \\mathbb{\\hat{E}}\\left[ D_{f}(\\pi_{\\theta}, \\pi_{\\theta_{old}})\\right] \\leq \\epsilon \\\\\n",
    "\\end{aligned}\n",
    "\\qquad\\Longleftrightarrow\\qquad\n",
    "\\begin{aligned}[c]\n",
    "\\max_{\\theta} \\quad & J(\\pi_\\theta) \\approx \\nabla_{\\theta} J(\\pi_\\theta) (\\theta - \\theta_{old}) \\\\\n",
    "\\text{s.t.: } \\quad & \\mathbb{\\hat{E}}\\left[ D_{f}(\\pi_{\\theta}, \\theta_{old} )\\right] \\approx \\frac{1}{2}(\\theta-\\theta_{old})^TF(\\theta-\\theta_{old}) \\leq \\epsilon \\\\\n",
    "\\end{aligned} \n",
    "\\end{equation*}\n",
    "\n",
    "**3.2 Lagrangian Function**\n",
    "\\begin{equation*}\n",
    "\\begin{aligned}[c]\n",
    "L(\\pi_{\\theta}, \\eta) = \\mathbb{\\hat{E}}\\left[ \\frac{\\pi_{\\theta}(a_t | s_t)}{\\pi_{\\theta_{old}}(a_t | s_t)} \\hat{A}_t\\right]  +\\eta \\left(\\epsilon - \\mathbb{\\hat{E}}\\left[ D_{f}( \\pi_{\\theta}, \\pi_{\\theta_{old}})\\right]  \\right) \n",
    "\\end{aligned}\n",
    "\\qquad\\Longleftrightarrow\\qquad\n",
    "\\begin{aligned}[c]\n",
    "L(\\theta, \\eta) = \\nabla_{\\theta} J(\\pi_\\theta) (\\theta - \\theta_{old}) + \\eta \\left(\\epsilon - \\frac{1}{2}(\\theta-\\theta_{old})^TF(\\theta-\\theta_{old})  \\right)\n",
    "\\end{aligned} \n",
    "\\end{equation*}\n",
    "\n"
   ]
  },
  {
   "cell_type": "markdown",
   "metadata": {},
   "source": [
    "> * 1. Calculate $\\partial_{\\pi_{\\theta}} L(\\pi_{\\theta}, \\eta)$\n",
    "\\begin{align}\n",
    "\\partial_{\\pi_{\\theta}} L(\\pi_{\\theta}, \\eta) &= \\frac{\\partial}{\\partial_{\\pi_{\\theta}}} \\left( \\mathbb{\\hat{E}}\\left[ \\frac{\\pi_{\\theta}}{\\pi_{\\theta_{old}}} \\hat{A}_t\\right]  +\\eta \\left( \\epsilon - \\mathbb{\\hat{E}}\\left[  D_{f}(\\pi_{\\theta}, \\pi_{\\theta_{old}})\\right]\\right)  \\right) \\\\\n",
    "&= \\frac{\\partial}{\\partial_{\\pi_{\\theta}}} \\left( \\mathbb{\\hat{E}}[\\frac{\\pi_{\\theta}}{\\pi_{\\theta_{old}}}\\hat{A}] - \\eta \\sum_i \\pi_{\\theta_{old}} f(\\frac{\\pi_{\\theta}}{\\pi_{\\theta_{old}}}) + \\eta \\epsilon\\right) \\\\\n",
    "&= \\left( \\sum_i \\left[\\frac{\\hat{A}}{\\pi_{\\theta_{old}}}\\right] - \\eta \\sum_i f'(\\frac{\\pi_{\\theta}}{\\pi_{\\theta_{old}}}) + 0 \\right) \\\\\n",
    "&= \\left( \\sum_i \\left[\\frac{\\hat{A}}{\\pi_{\\theta_{old}}}\\right] - \\eta \\sum_i ( \\frac{1}{\\alpha-1} (\\frac{\\pi_{\\theta}}{\\pi_{\\theta_{old}}})^{\\alpha-2} + \\frac{1}{\\pi_{\\theta_{old}}} )\\right) \\\\\n",
    "&= ?\n",
    "\\end{align}\n",
    "* 2. Calculate $\\partial_{\\theta} L(\\theta, \\eta)$\n",
    "\\begin{align}\n",
    "\\frac{\\partial}{\\partial \\theta} L(\\theta, \\eta) &= \\nabla_{\\theta} J(\\pi_\\theta) (\\theta - \\theta_{old}) + \\eta \\left(  \\epsilon - \\frac{1}{2}(\\theta-\\theta_{old})^TF(\\theta-\\theta_{old}) \\right) \\\\\n",
    "&= \\nabla_{\\theta}J(\\pi_\\theta) - \\eta F(\\theta - \\theta_{old}) \\\\\n",
    "&= 0 \\\\\n",
    "\\Rightarrow \\theta - \\theta_{old} &= \\frac{1}{\\eta}F^{-1} \\nabla_{\\theta} J(\\pi_{\\theta}) \n",
    "\\end{align}"
   ]
  },
  {
   "cell_type": "code",
   "execution_count": null,
   "metadata": {},
   "outputs": [],
   "source": []
  }
 ],
 "metadata": {
  "kernelspec": {
   "display_name": "Python 3",
   "language": "python",
   "name": "python3"
  },
  "language_info": {
   "codemirror_mode": {
    "name": "ipython",
    "version": 3
   },
   "file_extension": ".py",
   "mimetype": "text/x-python",
   "name": "python",
   "nbconvert_exporter": "python",
   "pygments_lexer": "ipython3",
   "version": "3.6.5"
  }
 },
 "nbformat": 4,
 "nbformat_minor": 2
}
